PropositionalLogic/Sound_Kripke.v
@@ -14,7 +14,7 @@ Require Import Logic.PropositionalLogic.GodelDummettLogic.
 Local Open Scope logic_base.
 Local Open Scope PropositionalLogic.
 
-Lemma sound_modus_ponens {L: Language} {nL: NormalLanguage L} {pL: PropositionalLanguage L} {SM: Semantics L} {pkS: PreKripkeSemantics L SM} {kiSM: KripkeIntuitionisticSemantics L SM}:
+Lemma sound_modus_ponens {L: Language} {nL: NormalLanguage L} {pL: PropositionalLanguage L} {SM: Semantics L} {pkSM: PreKripkeSemantics L SM} {kiM: KripkeIntuitionisticModel L SM} {kiSM: KripkeIntuitionisticSemantics L SM}:
   forall x y: expr,
     forall M m,
       KRIPKE: M, m |= (x --> y) -> KRIPKE: M, m |= x -> KRIPKE: M, m |= y.
@@ -27,7 +27,7 @@ Proof.
   reflexivity.
 Qed.
 
-Lemma sound_axiom1 {L: Language} {nL: NormalLanguage L} {pL: PropositionalLanguage L} {SM: Semantics L} {pkS: PreKripkeSemantics L SM} {kiSM: KripkeIntuitionisticSemantics L SM}:
+Lemma sound_axiom1 {L: Language} {nL: NormalLanguage L} {pL: PropositionalLanguage L} {SM: Semantics L} {pkSM: PreKripkeSemantics L SM} {kiM: KripkeIntuitionisticModel L SM} {kiSM: KripkeIntuitionisticSemantics L SM}:
   forall x y: expr,
     forall M m,
       KRIPKE: M, m |= x --> y --> x.
@@ -38,7 +38,7 @@ Proof.
   eapply sat_mono; eauto.
 Qed.
 
-Lemma sound_axiom2 {L: Language} {nL: NormalLanguage L} {pL: PropositionalLanguage L} {SM: Semantics L} {pkS: PreKripkeSemantics L SM} {kiSM: KripkeIntuitionisticSemantics L SM}:
+Lemma sound_axiom2 {L: Language} {nL: NormalLanguage L} {pL: PropositionalLanguage L} {SM: Semantics L} {pkSM: PreKripkeSemantics L SM} {kiM: KripkeIntuitionisticModel L SM} {kiSM: KripkeIntuitionisticSemantics L SM}:
   forall x y z: expr,
     forall M m,
       KRIPKE: M, m |= (x --> y --> z) --> (x --> y) --> (x --> z).
@@ -61,7 +61,7 @@ Proof.
   auto.
 Qed.
 
-Lemma sound_andp_intros {L: Language} {nL: NormalLanguage L} {pL: PropositionalLanguage L} {SM: Semantics L} {pkS: PreKripkeSemantics L SM} {kiSM: KripkeIntuitionisticSemantics L SM}:
+Lemma sound_andp_intros {L: Language} {nL: NormalLanguage L} {pL: PropositionalLanguage L} {SM: Semantics L} {pkSM: PreKripkeSemantics L SM} {kiM: KripkeIntuitionisticModel L SM} {kiSM: KripkeIntuitionisticSemantics L SM}:
   forall x y: expr,
     forall M m,
       KRIPKE: M, m |= x --> y --> x && y.
@@ -75,7 +75,7 @@ Proof.
   + auto.
 Qed.
 
-Lemma sound_andp_elim1 {L: Language} {nL: NormalLanguage L} {pL: PropositionalLanguage L} {SM: Semantics L} {pkS: PreKripkeSemantics L SM} {kiSM: KripkeIntuitionisticSemantics L SM}:
+Lemma sound_andp_elim1 {L: Language} {nL: NormalLanguage L} {pL: PropositionalLanguage L} {SM: Semantics L} {pkSM: PreKripkeSemantics L SM} {kiM: KripkeIntuitionisticModel L SM} {kiSM: KripkeIntuitionisticSemantics L SM}:
   forall x y: expr,
     forall M m,
       KRIPKE: M, m |= x && y --> x.
@@ -86,7 +86,7 @@ Proof.
   tauto.
 Qed.
 
-Lemma sound_andp_elim2 {L: Language} {nL: NormalLanguage L} {pL: PropositionalLanguage L} {SM: Semantics L} {pkS: PreKripkeSemantics L SM} {kiSM: KripkeIntuitionisticSemantics L SM}:
+Lemma sound_andp_elim2 {L: Language} {nL: NormalLanguage L} {pL: PropositionalLanguage L} {SM: Semantics L} {pkSM: PreKripkeSemantics L SM} {kiM: KripkeIntuitionisticModel L SM} {kiSM: KripkeIntuitionisticSemantics L SM}:
   forall x y: expr,
     forall M m,
       KRIPKE: M, m |= x && y --> y.
@@ -97,7 +97,7 @@ Proof.
   tauto.
 Qed.
 
-Lemma sound_orp_intros1 {L: Language} {nL: NormalLanguage L} {pL: PropositionalLanguage L} {SM: Semantics L} {pkS: PreKripkeSemantics L SM} {kiSM: KripkeIntuitionisticSemantics L SM}:
+Lemma sound_orp_intros1 {L: Language} {nL: NormalLanguage L} {pL: PropositionalLanguage L} {SM: Semantics L} {pkSM: PreKripkeSemantics L SM} {kiM: KripkeIntuitionisticModel L SM} {kiSM: KripkeIntuitionisticSemantics L SM}:
   forall x y: expr,
     forall M m,
       KRIPKE: M, m |= x --> x || y.
@@ -108,7 +108,7 @@ Proof.
   tauto.
 Qed.
 
-Lemma sound_orp_intros2 {L: Language} {nL: NormalLanguage L} {pL: PropositionalLanguage L} {SM: Semantics L} {pkS: PreKripkeSemantics L SM} {kiSM: KripkeIntuitionisticSemantics L SM}:
+Lemma sound_orp_intros2 {L: Language} {nL: NormalLanguage L} {pL: PropositionalLanguage L} {SM: Semantics L} {pkSM: PreKripkeSemantics L SM} {kiM: KripkeIntuitionisticModel L SM} {kiSM: KripkeIntuitionisticSemantics L SM}:
   forall x y: expr,
     forall M m,
       KRIPKE: M, m |= y --> x || y.
@@ -119,7 +119,7 @@ Proof.
   tauto.
 Qed.
 
-Lemma sound_orp_elim {L: Language} {nL: NormalLanguage L} {pL: PropositionalLanguage L} {SM: Semantics L} {pkS: PreKripkeSemantics L SM} {kiSM: KripkeIntuitionisticSemantics L SM}:
+Lemma sound_orp_elim {L: Language} {nL: NormalLanguage L} {pL: PropositionalLanguage L} {SM: Semantics L} {pkSM: PreKripkeSemantics L SM} {kiM: KripkeIntuitionisticModel L SM} {kiSM: KripkeIntuitionisticSemantics L SM}:
   forall x y z: expr,
     forall M m,
       KRIPKE: M, m |= (x --> z) --> (y --> z) --> (x || y --> z).
@@ -138,7 +138,7 @@ Proof.
     apply H2; auto.
 Qed.
 
-Lemma sound_falsep_elim {L: Language} {nL: NormalLanguage L} {pL: PropositionalLanguage L} {SM: Semantics L} {pkS: PreKripkeSemantics L SM} {kiSM: KripkeIntuitionisticSemantics L SM}:
+Lemma sound_falsep_elim {L: Language} {nL: NormalLanguage L} {pL: PropositionalLanguage L} {SM: Semantics L} {pkSM: PreKripkeSemantics L SM} {kiM: KripkeIntuitionisticModel L SM} {kiSM: KripkeIntuitionisticSemantics L SM}:
   forall x: expr,
     forall M m,
       KRIPKE: M, m |= FF --> x.
@@ -149,7 +149,7 @@ Proof.
   tauto.
 Qed.
 
-Lemma sound_excluded_middle_ident {L: Language} {nL: NormalLanguage L} {pL: PropositionalLanguage L} {SM: Semantics L} {pkS: PreKripkeSemantics L SM} {kiSM: KripkeIntuitionisticSemantics L SM}:
+Lemma sound_excluded_middle_ident {L: Language} {nL: NormalLanguage L} {pL: PropositionalLanguage L} {SM: Semantics L} {pkSM: PreKripkeSemantics L SM} {kiM: KripkeIntuitionisticModel L SM} {kiSM: KripkeIntuitionisticSemantics L SM}:
   forall x: expr,
     forall M,
       (forall m n, @Korder _ _ _ _ _ _ M m n -> m = n) ->
@@ -164,7 +164,7 @@ Proof.
   tauto.
 Qed.
 
-Lemma sound_impp_choice_no_branch {L: Language} {nL: NormalLanguage L} {pL: PropositionalLanguage L} {SM: Semantics L} {pkS: PreKripkeSemantics L SM} {kiSM: KripkeIntuitionisticSemantics L SM}:
+Lemma sound_impp_choice_no_branch {L: Language} {nL: NormalLanguage L} {pL: PropositionalLanguage L} {SM: Semantics L} {pkSM: PreKripkeSemantics L SM} {kiM: KripkeIntuitionisticModel L SM} {kiSM: KripkeIntuitionisticSemantics L SM}:
   forall x y: expr,
     forall M,
       (forall m1 m2 n, @Korder _ _ _ _ _ _ M m1 n -> @Korder _ _ _ _ _ _ M m2 n -> @Korder _ _ _ _ _ _ M m1 m2 \/ @Korder _ _ _ _ _ _ M m2 m1) ->
